<?xml version="1.0" encoding="UTF-8"?>
<exercises xmlns:xi="http://www.w3.org/2001/XInclude" xml:id="practice-sec-induction">

<title>Practice Problems</title>




  <exercise label="ind-mc-induction-step">
    <statement>
      <p>
        Suppose you are trying to prove, by mathematical induction, that a statement <m>P(n)</m> is true for all <m>n \ge 0</m>.  What would you attempt to prove in the <em>induction step</em> of the proof?  (Select all that apply.)
      </p>
    </statement>
    <choices randomize="yes">
      <choice correct="yes">
        <statement>
          <p>
            That assuming <m>P(k)</m> is true for an arbitrary <m>k \ge 0</m>, we can prove that <m>P(k+1)</m> is true.
          </p>
        </statement>
      </choice>
      <choice correct="yes">
        <statement>
          <p>
            That <m>P(k)</m> implies <m>P(k+1)</m> for all <m>k \ge 0</m>.
          </p>
        </statement>
      </choice>
      <choice>
        <statement>
          <p>
            That assuming <m>P(k+1)</m> is true for an arbitrary <m>k \ge 0</m>, we can prove that <m>P(k)</m> is true.
          </p>
        </statement>
      </choice>
      <choice correct="no">
        <statement>
          <p>
            That <m>P(k+1)</m> implies <m>P(k)</m> for all <m>k \ge 0</m>.
          </p>
        </statement>
      </choice>
      <choice correct="no">
        <statement>
          <p>
            That <m>P(k)</m> implies <m>P(k+1)</m> for at least one <m>k \ge 0</m>.
          </p>
        </statement>
      </choice>
    </choices>
  </exercise>

  <exercise label="ind-mc-steps1">
    <statement>
      <p>
        Suppose you wanted to prove the following statement:
        <me>
          2 + 4 + 6 + \cdots + 2n = n(n+1) \text{ for all } n \ge 1
        </me>.
        What would the first line of a proof by induction be?
      </p>
    </statement>
    <choices randomize="yes">
      <choice correct="yes">
        <statement>
          <p>
            Let <m>P(n)</m> be the statement <q><m>2 + 4 + 6 + \cdots + 2n = n(n+1)</m>.</q>
          </p>
        </statement>
      </choice>
      <choice>
        <statement>
          <p>
            Let <m>P(n)</m> be the statement <q><m>2 + 4 + 6 + \cdots + 2n = n(n-1)</m> for all <m>n \ge 1</m>.</q>
          </p>
        </statement>
      </choice>
      <choice>
        <statement>
          <p>
            Assume <m>P(n)</m> is true for all <m>n \ge 1</m>.
          </p>
        </statement>
      </choice>
      <choice>
        <statement>
          <p>
            Let <m>P(n) = 2 + 4 + 6 + \cdots + 2n</m>.
          </p>
        </statement>
      </choice>
      <choice>
        <statement>
          <p>
            Suppose <m>P(n) = n(n+1)</m> for all <m>n \ge 1</m>.
          </p>
        </statement>
      </choice>
    </choices>
  </exercise>


  <exercise label="ind-mc-steps2">
    <statement>
      <p>
        Suppose you were proving the following statement by mathematical induction:
        <me>
          2 + 4 + 6 + \cdots + 2n = n(n+1) \text{ for all } n \ge 1
        </me>.
        What would you need to show to establish the base case?
      </p>
    </statement>
    <choices randomize="yes">
      <choice correct="yes">
        <statement>
          <p>
            Show that <m>P(1)</m> is true.  That is, show that <m>2 = 1(1+1)</m>.
          </p>
        </statement>
      </choice>
      <choice>
        <statement>
          <p>
            Show that <m>P(2)</m> is true.  That is, show that <m>2 + 4 = 2(2+1)</m>.
          </p>
        </statement>
        <feedback>
          <p>
            Even though the sum starts with <m>2</m>, we need to consider the smallest <m>n</m> for which the statement <m>P(n)</m> is true.
          </p>
        </feedback>
      </choice>
      <choice>
        <statement>
          <p>
            Show that <m>P(1)</m> and <m>P(2)</m> are both true.
          </p>
        </statement>
      </choice>
      <choice>
        <statement>
          <p>
            Show that <m>P(1)</m> implies <m>P(2)</m>.
          </p>
        </statement>
      </choice>
      <choice>
        <statement>
          <p>
            Nothing, since the sum already has more than <m>n = 1</m> terms.
          </p>
        </statement>
      </choice>
    </choices>
  </exercise>

  <exercise label="ind-mc-steps3">
    <statement>
      <p>
        Suppose you were proving the following statement by mathematical induction:
        <me>
          2 + 4 + 6 + \cdots + 2n = n(n+1) \text{ for all } n \ge 1
        </me>.
        What would the first line of the inductive case be?
      </p>
    </statement>
    <choices randomize="yes">
      <choice correct="yes">
        <statement>
          <p>
            Assume <m>P(k)</m> is true for some arbitrary <m>k \ge 1</m>, that is, assume <m>2+4+6+\cdots + 2k = k(k+1)</m>.
          </p>
        </statement>
      </choice>
      <choice>
        <statement>
          <p>
            Assume <m>P(k)</m> is true for all <m>k \ge 1</m>, that is, assume <m>2+4+6+\cdots + 2k = k(k+1)</m>.
          </p>
        </statement>
        <feedback>
          <p>
            Assume <m>P(k)</m> and <m>P(k)</m> are both true for an arbitrary <m>k \ge 1</m>; that is, assume <m>2+4+6+\cdots + 2k = k(k+1)</m> and <m>2+4+6+\cdots + 2k+ 2k+2) = (k+1)(k+2)</m>.
          </p>
        </feedback>
      </choice>
      <choice>
        <statement>
          <p>
            Assume <m>P(k)</m> implies <m>P(k+1)</m> for an arbitrary <m>k \ge 1</m>.
          </p>
        </statement>
      </choice>
      <choice>
        <statement>
          <p>
            Assume <m>P(k)</m> is true for some large <m>k \ge 1</m>; say, assume <m>2 + 4 + 6 + \cdots + 432 = 216(217)</m>.
          </p>
        </statement>
      </choice>

    </choices>
  </exercise>
  
  <exercise label="ind-drag-recurrence" >
    <statement>
      <p>
        Arrange some of the statements below to create a correct proof by induction that the recurrence relation <m>a_n = 5a_{n-1} + 4</m>, with initial condition <m>a_0 = 0</m> has closed formula <m>a_n = 5^n - 1</m>.
      </p>
    </statement>
    <blocks>
    <block order="2">
    <p>
      Let <m>P(n)</m> be the statement, <q><m>a_n = 5^n - 1</m></q>.
    </p>
    </block>
    <block order="4">

    <p>
      Note that <m>a_0 = 5^0 - 1 = 0</m>, so <m>P(0)</m> is true.
    </p>
    </block>
    <block order="5">
    <p>
      Now assume that <m>P(k)</m> is true for an arbitrary integer <m>k \ge 0</m>.
    </p>
    </block>
    <block order="1">
    <p>
      Then <m>a_k = 5^k - 1</m>.
    </p>
    </block>
    <block order="3">
    <p>
      By the recurrence relation, we have <m>a_{k+1} = 5 a_k + 4 = 5 (5^k -1) + 4</m>.
    </p>
    </block>
    <block>
      <p>
        This simplifies to <m>a_{k+1} = 5^{k+1} - 5 + 4 = 5^{k+1} - 1</m>, so <m>P(k+1)</m> is true.
      </p>
    </block>
    <block>
      <p>
        Therefore, by the principle of mathematical induction, <m>P(n)</m> is true for all <m>n \ge 0</m>.
      </p>
    </block>
    <block correct="no">
      <p>
        Now assume that <m>P(k+1)</m> is true for an arbitrary integer <m>k \ge 0</m>.
      </p>
    </block>
    <block correct="no">
      <p>
        Then <m>a_{k+1} = 5a_k+4</m>, so <m>P(k+1)</m> is true.
      </p>
    </block>
    </blocks>
  </exercise>


  <exercise label="ind-drag-multiple" >
    <statement>
      <p>
        Arrange some of the statements below to create a correct proof by induction that for all <m>n \ge 1</m>, the number <m>14^n - 1</m> is a multiple of <m>13</m>. 
      </p>
    </statement>
    <blocks>
    <block order="2">
    <p>
      Let <m>P(n)</m> be the statement, <q><m>14^n - 1</m> is a multiple of <m>13</m>.</q>
    </p>
    </block>
    <block order="4">
    <p>
      Note that <m>14^1 - 1 = 13</m>, so this is definitely a multiple of <m>13</m>.
    </p>
    </block>
    <block order="5">
    <p>
      Now assume that <m>P(k)</m> is true for an arbitrary integers <m>k \ge 1</m>.
    </p>
    </block>
    <block>
      <p>
        Then <m>14^k - 1 = 13\cdot j</m> for some integer <m>j</m>.
      </p>
    </block>
    <block order="1">
    <p>
      Since <m>14^{k+1} - 1 = 14(14^k - 1) + 14 - 1 = 14(13\cdot j) + 13</m>, we see that <m>14^{k+1} - 1</m> is a multiple of <m>13</m>.
    </p>
    </block>
    <block order="3">
    <p>
      Thus <m>P(k+1)</m> is true.
    </p>
    </block>
    <block>
      <p>
        Therefore, by the principle of mathematical induction, <m>P(n)</m> is true for all <m>n \ge 1</m>.
      </p>
    </block>
    <block correct="no">
      <p>
        Note that <m>14^2 - 1 = (14-1)(14+1)</m> by difference of squares, so this is a multiple of 13.
      </p>
    </block>
    <block correct="no">
      <p>
        Now assume that <m>P(n)</m> is true for all <m>n \ge 1</m>.
      </p>
    </block>
    <block correct="no">
      <p>
        Thus <m>14^k = \frac{14^{k+1} - 1}{14}</m>, which must also be a multiple of 13.
      </p>
    </block>
    </blocks>
  </exercise>


  <exercise label="ind-drag-sum" >
    <statement>
      <p>
        Arrange some of the statements below to create a correct proof by induction that for all <m>n \ge 1</m>, <m>1+1+2+3+5+\cdots + F_n = F_{n+2} - 1</m>, where <m>F_n</m> is the <m>n</m>th Fibonacci number.
      </p>
    </statement>
    <blocks>
    <block order="2">
    <p>
      Let <m>P(n)</m> be the statement, <q><m>1+1+2+3+5+\cdots + F_n = F_{n+2} - 1</m>.</q>
    </p>
    </block>
    <block order="4">

    <p>
      For the base case, note that <m>P(1)</m> and <m>P(2)</m> are true, because <m>1 = 2-1</m> and <m>1+1 = 3-1</m>.
    </p>
    </block>
    <block order="5">
    <p>
      Now assume that <m>P(k)</m> is true for an arbitrary integer <m>k \ge 2</m>.
    </p>
    </block>
    <block order="1">
    <p>
      That is, assume <m>1+1+2+3 + 5+F_k = F_{k+2} - 1</m>.
    </p>
    </block>
    <block order="3">
    <p>
      Then adding <m>F_{k+1}</m> to both sides, we get <m>1+1+2+3+5+\cdots + F_k + F_{k+1} = F_{k+1} + F_{k+2} - 1</m>.
    </p>
    </block>
    <block>
      <p>
        By the definition of Fibonacci numbers, <m>F_{k+1} + F_{k+2} = F_{k+3}</m>, so the right-hand side simplifies to <m>F_{k+3} - 1</m>.
      </p>
    </block>
    <block order="2">
      <p>
        Thus <m>P(k+1)</m> is true, and therefore by the principle of mathematical induction, <m>P(n)</m> is true for all <m>n \ge 1</m>.
      </p>
    </block>
    <block correct="no" order="1">
      <p>
        For the base case, note that <m>1+1+2 = 4 = F_{5}-1</m>.
      </p>
    </block>
    <block correct="no">
      <p>
        Then by the inductive hypothesis, <m>1+1+2+3+\cdots+F_{k+1} = F_{k+2} - 1</m>.
      </p>
    </block>
    <block correct="no" order="7">
      <p>
        Subtracting <m>F_{k+1}</m> from both sides gives us <m>P(k)</m>, which we also assumed to be true.
      </p>
    </block>

    </blocks>
  </exercise>

</exercises>
